#mar1
#### Verify

$\frac{\cot(\theta)}{\csc(\theta)} = \cos(\theta)$
$\frac{\frac{\cos(\theta)}{\sin(\theta)}}{\frac{1}{\sin(\theta)}} = \cos(\theta)$
$\frac{\cos(\theta)}{\sin(\theta)} * {\frac{\sin(\theta)}{1}} = \cos(\theta)$
$\frac{\cos(\theta)\sin(\theta)}{\sin(\theta)} = \cos(\theta)$
$\cos(\theta)=\cos(\theta)$

---
$\csc(\alpha)\tan(\alpha)=\sec(\alpha)$
$\tan(\alpha)=\frac{\sec(\alpha)}{\csc(\theta)}$
$\tan(\alpha)=\frac{\frac{1}{\cos(\alpha)}}{\frac{1}{\sin(\alpha)}}$
$\tan(\alpha)=\frac{1}{\cos(\alpha)}*\frac{\sin(\alpha)}{1}$
$\tan(\alpha)=\frac{\sin(\alpha)}{\cos(\alpha)}$
$\tan(\alpha)=\tan(\alpha\therefore \csc(\alpha)\tan(\alpha))=\sec(\alpha)$

---

$\frac{\cos(m)}{1+\sin(m)}=\frac{1-\sin(m)}{\cos(m)}$
$\frac{1-\sin(m)}{1-\sin(m)} * \frac{\cos(m)}{1+\sin(m)}=\frac{1-\sin(m)}{\cos(m)}$
$\frac{\cos(m)-\cos(m)\sin(m)}{1-\sin^2(m)}=\frac{1-\sin(m)}{\cos(m)}$
$\frac{\cos(m)-\cos(m)\sin(m)}{\cos^2(m)}=\frac{1-\sin(m)}{\cos(m)}$
$\frac{\cos(m)(1-\sin(m))}{\cos^2(m)}=\frac{1-\sin(m)}{\cos(m)}$
$\frac{1-\sin(m)}{\cos(m)}=\frac{1-\sin(m)}{\cos(m)}$

---

$$\frac{1+\sin(\lambda)}{\sin(\lambda)}+\frac{\cot(\lambda)-\cos(\lambda)}{\cos(\lambda)} = \frac{2}{\sin(\lambda)}$$
$$\frac{1+\sin(\lambda)}{\sin(\lambda)}+\frac{\cot(\lambda)-\cos(\lambda)}{\cos(\lambda)} = 2\csc(\lambda)$$
$$\frac{\cos(\lambda)+\sin(\lambda)\cos(\lambda)}{\sin(\lambda)\cos(\lambda)}+\frac{\cot(\lambda)\sin(\lambda)-\cos(\lambda)\sin(\lambda)}{\cos(\lambda)\sin(\lambda)} = 2\csc(\lambda)$$
$$\frac{\cos(\lambda)+\sin(\lambda)\cos(\lambda)+\frac{\cos(\lambda)}{\sin(\lambda)}\sin(\lambda)-\cos(\lambda)\sin(\lambda)}{\sin(\lambda)\cos(\lambda)} = 2\csc(\lambda)$$
$$\frac{\cos(\lambda)+\frac{\cos(\lambda)}{\sin(\lambda)}\sin(\lambda)}{\sin(\lambda)\cos(\lambda)} = 2\csc(\lambda)$$
$$\frac{\cos(\lambda)+\frac{\cos(\lambda)\sin(\lambda)}{\sin(\lambda)}}{\sin(\lambda)\cos(\lambda)} = 2\csc(\lambda)$$
$$\frac{\cos(\lambda)+\cos(\lambda)}{\sin(\lambda)\cos(\lambda)} = 2\csc(\lambda)$$$$\frac{2\cos(\lambda)}{\sin(\lambda)\cos(\lambda)} = 2\csc(\lambda)$$
$$\frac{2}{\sin(\lambda)} = 2\csc(\lambda)$$
$$2\csc(\lambda) = 2\csc(\lambda)$$
---


