#mar4 #trig

#### Double Angles:

$\cos(2\theta)=\cos^2(\theta)-\sin^2(\theta)$
	  $\space=2\cos^2(\theta)-1$
	  $\space=1-2\sin^2(\theta)$

$\sin(2\theta)=2\sin(\theta)\cos(\theta)$

$\tan(2\theta)=\frac{2\tan(\theta)}{1-\tan^2(\theta)}$

---

#### Proof of Double Angle Identities
$\cos(2\alpha) = \cos(\alpha+\alpha)$

$\cos(\alpha+\beta) = \cos(\alpha)\cos(\beta)-\sin(\alpha)\sin(\beta)$   | [[7.5 Sum and Difference Identities]]

$\cos(\alpha+\alpha) = \cos(\alpha)\cos(\alpha)-\sin(\alpha)\sin(\alpha)$ 
> $\cos(2\alpha) = \cos^2(\alpha)-\sin^2(\alpha)$ 

$\sin^2(\theta) + \cos^2(\theta) = 1$ | [[6.3 Properties of Trig Functions]]
$\sin^2(\theta)= 1-\cos^2(\theta)$

$\cos(\alpha+\alpha) = \cos^2(\alpha)-(1-\cos^2(\alpha))$ 
$\cos(\alpha+\alpha) = \cos^2(\alpha)-1+\cos^2(\alpha))$ 
> $\cos(2\alpha) = 2\cos^2(\alpha)-1$ 

$\cos^2(\theta) = 1-\sin^2(\theta)$
 $\cos(\alpha+\alpha) = 1-\sin^2(\alpha)-\sin^2(\alpha)$ 
> $\cos(2\alpha) = 1-2\sin^2(\alpha)$ 



$\sin(2\alpha) = \sin(\alpha+\alpha)$
$= \sin(\alpha)\cos(\alpha)+\cos(\alpha)\sin(\alpha)$
> $= 2\sin(\alpha)\cos(\alpha)$

$\tan(2\alpha) = \tan(\alpha+\alpha)$
$=\frac{\tan(\alpha)+\tan(\alpha)}{1-\tan(\alpha)\tan(\alpha)}$
> $=\frac{2\tan(\alpha)}{1-\tan^2(\alpha)}$

---

#### Half Angles:
$\cos(\frac{\theta}{2})=\pm\sqrt{\frac{1+\cos(\theta)}{2}}$
$\sin(\frac{\theta}{2})=\pm\sqrt{\frac{1-\cos(\theta)}{2}}$
$\tan(\frac{\alpha}{2}) =\pm\sqrt{\frac{1-\cos(\alpha)}{1+\cos(\alpha)}}$


---

$\text{if: } \cos(2\alpha) = 2\cos^2(\alpha)-1 \therefore \cos(\alpha)=2\cos^2(\frac{\alpha}{2})-1$

Solve for $\frac{\alpha}{2}$
$\cos(\alpha)=2\cos^2(\frac{\alpha}{2})-1$
$\cos(\alpha)+1=2\cos^2(\frac{\alpha}{2})$
$\frac{\cos(\alpha)+1}{2}=\cos^2(\frac{\alpha}{2})$

$\cos^2(\frac{\alpha}{2})=\frac{\cos(\alpha)+1}{2}$
> $\cos(\frac{\alpha}{2})=\pm\sqrt{\frac{1+\cos(\alpha)}{2}}$




Using:
$\cos(\alpha)=2\cos^2(\frac{\alpha}{2})-1$

$\cos(\alpha)+1=2\cos^2(\frac{\alpha}{2})$
$\cos(\alpha)+1=2(1-\sin^2(\alpha))$
$\cos(\alpha)+1=2-2\sin^2(\alpha))$

$\frac{\cos(\alpha)-1}{-2}=\sin^2(\alpha)$
$\frac{-\cos(\alpha)+1}{2}=\sin^2(\alpha)$
$\sin^2(\alpha)=\frac{1-\cos(\alpha)}{2}$
$\sin(\alpha)=\pm\sqrt{\frac{1-\cos(\alpha)}{2}}$
